Dodanie jednoznaczności odwrotności

main.v
@@ -9,11 +9,10 @@ Record GroupTheo : Type := groupTheo
     inv := forall(x : G), exists( e y : G) , op x y = e /\ op y x  = e; 
   }.
 
+(* Jednoznaczność elementu neutralnego *)
 Definition idPro (g : GroupTheo ) (e : G g) := (forall(x : G g), op g e x = x /\ op g x e = x).
 
-
 Theorem exOnlyOne : forall (g : GroupTheo), forall( e f : G g), (idPro g e /\ idPro g f) -> e = f.
-
 Proof.  
   unfold idPro.
   intros.
@@ -25,3 +24,42 @@ Proof.
   rewrite <- H2.
   trivial.
 Qed.
+
+(* Jednoznaczność elementu odwrotnego *)
+Definition invPro (g : GroupTheo) (e y : G g):= idPro g e /\ ( forall(x : G g) ,( op g x y = e /\ op g y x  = e)).
+
+Theorem exOnlyOneInv : forall( g : GroupTheo), forall (e y1 y2 x : G g), invPro g e y1 /\ invPro g e y2 -> y1 = y2.
+Proof.
+  unfold invPro.
+  unfold idPro.
+  intros.
+  destruct H.
+  destruct H.
+  destruct H0.
+  pose proof H y1.
+  destruct H3.
+  pose proof H y2.
+  destruct H5.
+  rewrite <- H4.
+  rewrite <- H5.
+  pose proof H1 x.
+  pose proof H2 x.
+  destruct H7.
+  destruct H8.
+  rewrite <- H8 at 1.
+  rewrite <- H9 at 1.
+  rewrite (assoc ).
+  trivial.
+Qed.
+
+
+Record Group : Type := group
+  { G : Set; (* nosnik *)
+    op : G -> G -> G; (* operacja *)
+    inv : G -> G;
+    e : G;
+  
+    assoc : forall(x y z : G), op (op x y) z = op x (op y z);
+    id :  forall(x : G), op e x = e /\ op x e = e ;
+    inverse :  forall(x : G), op x (inv x) = e /\ op (inv x) x  = e ;
+  }.
